@prefix :       	<https://ukfires.org/probs/ontology/> .
@prefix ufpc:   	<https://ukfires.org/probs/ontology/prodcom/> .
@prefix ufct:   	<https://ukfires.org/probs/ontology/comtrade/> .
@prefix beis:   	<https://ukfires.org/probs/ontology/beis/> .
@prefix cc:     	<http://creativecommons.org/ns#> .
@prefix dc:     	<http://purl.org/dc/elements/1.1/> .
@prefix gn:     	<http://www.geonames.org/ontology#> .
@prefix gnd:        <https://sws.geonames.org/> .
@prefix owl:    	<http://www.w3.org/2002/07/owl#> .
@prefix prov:   	<http://www.w3.org/ns/prov#> .
@prefix quantitykind:	<http://qudt.org/vocab/quantitykind/> .
@prefix qudt:		<http://qudt.org/schema/qudt/> .
@prefix rdf:    	<http://www.w3.org/1999/02/22-rdf-syntax-ns#> .
@prefix rdfs:   	<http://www.w3.org/2000/01/rdf-schema#> .
@prefix time:		<http://www.w3.org/2006/time#> .
@prefix vann:   	<http://purl.org/vocab/vann/> .
@prefix xml:    	<http://www.w3.org/XML/1998/namespace> .
@prefix xsd:    	<http://www.w3.org/2001/XMLSchema#> .
@base           	<https://ukfires.org/probs/ontology> .

<https://ukfires.org/probs/ontology>
    rdf:type            owl:Ontology ;

    rdfs:label          "Physical Resources Observatory (PRObs) Ontology"@en ;
    dc:title            "Physical Resources Observatory (PRObs) Ontology"@en ;

    rdfs:comment        "The ontology describes entities useful for the development of the Physical Resources Observatory (PRObs) data integration system"@en ;
    dc:description      "The ontology describes entities useful for the development of the Physical Resources Observatory (PRObs) data integration system"@en ;

    owl:versionIRI      <https://ukfires.org/probs/ontology-1.5.2> ;
    owl:versionInfo     "1.5.2" ;
    dc:issued           "2020-10-02" ;
    dc:modified         "2021-04-16" ;

    dc:creator          "UK FIRES partners"@en ;

    dc:contributor      "Stefano Germano" ;
    dc:contributor      "Rick Lupton" ;
    dc:contributor      "Carla Saunders" ;

    vann:preferredNamespacePrefix   "uf" ;
    vann:preferredNamespaceUri      "https://ukfires.org/probs/ontology" ;

    cc:licence          <https://creativecommons.org/licenses/by/4.0> .


#################################################################
#    Object Properties
#################################################################

:objectComposedOf
    rdf:type            owl:ObjectProperty ;
    rdfs:label          "object composed of"@en ;
    rdfs:comment        "Relation which connects an Object to sub-objects lower in the hierarchy"@en ;
    rdfs:domain         :Object ;
    rdfs:range          :Object .


:objectEquivalentTo
    rdf:type            owl:ObjectProperty ;
    rdf:type            owl:ReflexiveProperty ;
    rdf:type            owl:SymmetricProperty ;
    rdf:type            owl:TransitiveProperty ;
    rdfs:label          "object equivalent to"@en ;
    rdfs:comment        "Relation which connects two Objects which describe exacly the same thing. Example: Cement :objectEquivalentTo CementInCOMTRADE"@en ;
    rdfs:domain         :Object ;
    rdfs:range          :Object .


:belongsToList
    rdf:type            owl:ObjectProperty ;
    rdf:type            owl:FunctionalProperty ;
    rdfs:label          "belongs to list"@en ;
    rdfs:comment        "Each ClassificationCode belongs to a ClassificationCodeList. Example: 10.11.11.40 :belongsToList 2017PRODCOMlist"@en ;
    rdfs:domain         :ClassificationCode ;
    rdfs:range          :ClassificationCodeList .


:hasClassificationCode
    rdf:type            owl:ObjectProperty ;
    rdfs:label          "has classification code"@en ;
    rdfs:comment        "Links an Object to the ClassificationCode which describes it. Example: Object10.11.11.40 :hasClassificationCode 10.11.11.40 "@en ;
    rdfs:domain         :Object ;
    rdfs:range          :ClassificationCode .


:objectDefinedBy
    rdf:type            owl:ObjectProperty ;
    rdfs:label          "object defined by"@en ;
    rdfs:comment        "Link Observations to the Object they describe"@en ;
    rdfs:domain         :Observation ;
    rdfs:range          :Object .


:objectDirectlyDefinedBy
    rdf:type            owl:ObjectProperty ;
    rdfs:subPropertyOf  :objectDefinedBy ;
    rdfs:label          "object directly defined by"@en ;
    rdfs:comment        "Link direct Observations to the Object they describe"@en ;
    rdfs:domain         :DirectObservation ;
    rdfs:range          :Object .


:objectInferredDefinedBy
    rdf:type            owl:ObjectProperty ;
    rdfs:subPropertyOf  :objectDefinedBy ;
    rdfs:label          "object inferred defined by"@en ;
    rdfs:comment        "Link inferred Observations to the Object they describe"@en ;
    rdfs:domain         :InferredObservation ;
    rdfs:range          :Object .


:processDefinedBy
    rdf:type            owl:ObjectProperty ;
    rdfs:label          "process defined by"@en ;
    rdfs:comment        "Link Observations to the Process they describe"@en ;
    rdfs:domain         :Observation ;
    rdfs:range          :Process .

:hasTimePeriod
    rdf:type            owl:ObjectProperty ;
    rdf:type            owl:FunctionalProperty ;
    rdfs:label          "has time period"@en ;
    rdfs:comment        "Links Observation to the TimePeriod in which it was measured"@en ;
    rdfs:domain         :Observation ;
    rdfs:range          time:DateTimeDescription .

:hasRegion
    rdf:type            owl:ObjectProperty ;
    rdf:type            owl:FunctionalProperty ;
    rdfs:label          "has region"@en ;
    rdfs:comment        "Links Observation to the Region in which it was measured"@en ;
    rdfs:domain         :Observation ;
    rdfs:range          gn:Feature .


:partOfDataset
    rdf:type            owl:ObjectProperty ;
    rdf:type            owl:FunctionalProperty ;
    rdfs:label          "part of dataset"@en ;
    rdfs:comment        "Links Observation to the Dataset it is a part of"@en ;
    rdfs:domain         :Observation ;
    rdfs:range          :Dataset .


:processComposedOf
    rdf:type            owl:ObjectProperty ;
    rdfs:label          "process composed of"@en ;
    rdfs:comment        "Relation which connects an Process to sub-processes lower in the hierarchy"@en ;
    rdfs:domain         :Process ;
    rdfs:range          :Process .

:processEquivalentTo
    rdf:type            owl:ObjectProperty ;
    rdf:type            owl:ReflexiveProperty ;
    rdf:type            owl:SymmetricProperty ;
    rdf:type            owl:TransitiveProperty ;
    rdfs:label          "process equivalent to"@en ;
    rdfs:comment        "Relation which connects two Processes which describe exacly the same thing."@en ;
    rdfs:domain         :Process ;
    rdfs:range          :Process .


:hasRole
    rdf:type            owl:ObjectProperty ;
    rdfs:label          "has role"@en ;
    rdfs:comment        "Links an observation to the type of data represented by it"@en ;
    rdfs:domain         :Observation ;
    rdfs:range          :Role .


:consumes
    rdf:type            owl:ObjectProperty ;
    rdfs:label          "consumes"@en ;
    rdfs:comment        "What object process consumes (i.e., the input of a process)"@en ;
    rdfs:domain         :Process ;
    rdfs:range          :Object .


:produces
    rdf:type            owl:ObjectProperty ;
    rdfs:label          "produces"@en ;
    rdfs:comment        "What object process produces (i.e., the output of a process)"@en ;
    rdfs:domain         :Process ;
    rdfs:range          :Object .

:metric
    rdf:type            owl:ObjectProperty ;
    rdfs:label          "metric"@en ;
    rdfs:comment        "The way in which a measurement is quantified."@en ;
    rdfs:domain         :Observation ;
    rdfs:range          qudt:QuantityKind .


:bound
    rdf:type            owl:ObjectProperty ;
    rdfs:label          ""@en ;
    rdfs:comment        ""@en ;
    rdfs:domain         :Observation ;
    rdfs:range          :MeasurementBound .


#################################################################
#    Data properties
#################################################################

:objectName
    rdf:type            owl:DatatypeProperty ;
    rdf:type            owl:FunctionalProperty ;
    rdfs:label          "object name"@en ;
    rdfs:comment        "Links an Object to its human-readable name"@en ;
    rdfs:domain         :Object ;
    rdfs:range          xsd:string .


:objectDescription
    rdf:type            owl:DatatypeProperty ;
    rdf:type            owl:FunctionalProperty ;
    rdfs:label          "object description"@en ;
    rdfs:comment        "Links an Object to a human-readble description of that Object"@en ;
    rdfs:domain         :Object ;
    rdfs:range          xsd:string .


:processName
    rdf:type            owl:DatatypeProperty ;
    rdf:type            owl:FunctionalProperty ;
    rdfs:label          "process name"@en ;
    rdfs:comment        "Links a Process to its human-readable name"@en ;
    rdfs:domain         :Process ;
    rdfs:range          xsd:string .


:processDescription
    rdf:type            owl:DatatypeProperty ;
    rdf:type            owl:FunctionalProperty ;
    rdfs:label          "process description"@en ;
    rdfs:comment        "Links a Process to a human-readble description of that Object"@en ;
    rdfs:domain         :Process ;
    rdfs:range          xsd:string .


:codeName
    rdf:type            owl:DatatypeProperty ;
    rdf:type            owl:FunctionalProperty ;
    rdfs:label          "code name"@en ;
    rdfs:comment        "Links a ClassificationCode to its human-readable version"@en ;
    rdfs:domain         :ClassificationCode ;
    rdfs:range          xsd:string .


:codeDescription
    rdf:type            owl:DatatypeProperty ;
    rdf:type            owl:FunctionalProperty ;
    rdfs:label          "code description"@en ;
    rdfs:comment        "Links a ClassificationCode to a human-readable description of that Object, usually defined by the body which maintains the ClassificationCodeList"@en ;
    rdfs:domain         :ClassificationCode ;
    rdfs:range          xsd:string .


:measurement
    rdf:type            owl:DatatypeProperty ;
    rdf:type            owl:FunctionalProperty ;
    rdfs:label          "measurement"@en ;
    rdfs:comment        "The actual quantity of an Observation."@en ;
    rdfs:domain         :Observation ;
    rdfs:range          xsd:decimal .

:metricName
    rdf:type            owl:DatatypeProperty ;
    rdf:type            owl:FunctionalProperty ;
    rdfs:label          "metric name"@en ;
    rdfs:comment        "Links a Metric to its human-readable version"@en ;
    rdfs:domain         qudt:QuantityKind ;
    rdfs:range          xsd:string .

#################################################################
#    Classes
#################################################################

:Object
    rdf:type            owl:Class ;
    rdfs:subClassOf     prov:Entity ;
    rdfs:label          "Object"@en ;
    rdfs:comment        "What is flowing in a Flow, or accumulated in a Stock. This is a more general term that includes Goods and Substances, but also non-material things such as energy and services."@en .


:ReferenceObject
    rdf:type            owl:Class ;
    rdfs:subClassOf     :Object ;
    rdfs:label          "ReferenceObject"@en ;
    rdfs:comment        ""@en .


:ClassificationCode
    rdf:type            owl:Class ;
    rdfs:label          "Classification code"@en ;
    rdfs:comment        "A label within a ClassificationCodeList. Example: 10.11.11.40 in the 2017-18 PRODCOM list."@en .


ufpc:ClassificationCode
    rdf:type            owl:Class ;
    rdfs:subClassOf     :ClassificationCode ;
    rdfs:label          "PRODCOM classification code"@en ;
    rdfs:comment        "A label within a PRODCOM ClassificationCodeList"@en .

ufct:ClassificationCode
    rdf:type            owl:Class ;
    rdfs:subClassOf     :ClassificationCode ;
    rdfs:label          "COMTRADE classification code"@en ;
    rdfs:comment        "A label within a COMTRADE ClassificationCodeList."@en .


:ClassificationCodeList
    rdf:type            owl:Class ;
    rdfs:label          "Classification code list"@en ;
    rdfs:comment        "A set of ClassificationCodes. Example: the 2017-18 PRODCOM list or the 2018 HS classification."@en .


ufpc:ClassificationCodeList
    rdf:type            owl:Class ;
    rdfs:subClassOf     :ClassificationCodeList ;
    rdfs:label          "PRODCOM classification code list"@en ;
    rdfs:comment        "A set of PRODCOM ClassificationCodes, usually from a specific year. Example: the 2017-18 PRODCOM list."@en .

ufct:ClassificationCodeList
    rdf:type            owl:Class ;
    rdfs:subClassOf     :ClassificationCodeList ;
    rdfs:label          "COMTRADE classification code list"@en ;
    rdfs:comment        "A set of COMTRADE ClassificationCodes, usually from a specific year. Example: the 2018 HS classification."@en .


:Observation
    rdf:type            owl:Class ;
    rdfs:subClassOf     prov:Entity ;
    rdfs:label          "Observation"@en ;
    rdfs:comment        "One set of observed data. At minimum the set of Object, Measurement and Dataset, preferably TimePeriod, and Region."@en .


:Role
    rdf:type            owl:Class ;
    rdfs:label          "Role"@en ;
    rdfs:comment        "Type of data represented by the Observation"@en .


:Flow
    rdf:type            owl:Class ;
    rdfs:subClassOf     :Role ;
    rdfs:label          "Flow"@en ;
    rdfs:comment        "The Flow of an Object between processes or across Regions"@en .


:SoldProduction
    rdf:type            owl:Class ;
    rdfs:subClassOf     :Flow ;
    rdfs:label          "Sold production"@en ;
    rdfs:comment        "Defined by PRODCOM, as opposed to the goods that may have been produced within the factory boundary, but haven't yet left the factory gate."@en .


:Import
    rdf:type            owl:Class ;
    rdfs:subClassOf     :Flow ;
    rdfs:label          "Import"@en ;
    rdfs:comment        "A Flow which describes the Flow of an Object into the Region of interest"@en .


:Export
    rdf:type            owl:Class ;
    rdfs:subClassOf     :Flow ;
    rdfs:label          "Export"@en ;
    rdfs:comment        "A Flow which describes the Flow of an Object out of the Region of interest"@en .


:ProcessInput
    rdf:type            owl:Class ;
    rdfs:subClassOf     :Flow ;
    rdfs:label          "Process input"@en ;
    rdfs:comment        "The input to a Process"@en .


:ProcessOutput
    rdf:type            owl:Class ;
    rdfs:subClassOf     :Flow ;
    rdfs:label          "Process output observation"@en ;
    rdfs:comment        "The output from a Process"@en .


:Stock
    rdf:type            owl:Class ;
    rdfs:subClassOf     :Role ;
    rdfs:label          "Stock"@en ;
    rdfs:comment        "The accumulation of a Stock of an Object"@en .


:DirectObservation
    rdf:type            owl:Class ;
    rdfs:subClassOf     :Observation ;
    rdfs:label          "Direct observation"@en ;
    rdfs:comment        "An Observation directly derived from the data"@en .


:InferredObservation
    rdf:type            owl:Class ;
    rdfs:subClassOf     :Observation ;
    rdfs:label          "Inferred observation"@en ;
    rdfs:comment        "An Observation inferred from other Observations"@en .


:Process
    rdf:type            owl:Class ;
    rdfs:label          "Process"@en ;
    rdfs:comment        "One or more grouped operations in a system that can be defined and separated from others. A Process has an input of some Object(s) and an output of some Object(s)"@en .


:Dataset
    rdf:type            owl:Class ;
    rdfs:label          "Dataset"@en ;
    rdfs:comment        "A collection of observations. Example: the 2018 PRODCOM dataset."@en .

:MeasurementBound
    rdf:type            owl:Class ;
    rdfs:label          ""@en ;
    rdfs:comment        ""@en .

:LowerBound
    rdf:type            owl:NamedIndividual , :MeasurementBound ;
    rdfs:label          ""@en ;
    rdfs:comment        ""@en .

:UpperBound
    rdf:type            owl:NamedIndividual , :MeasurementBound ;
    rdfs:label          ""@en ;
    rdfs:comment        ""@en .

:ExactBound
    rdf:type            owl:NamedIndividual , :MeasurementBound ;
    rdfs:label          ""@en ;
    rdfs:comment        ""@en .
