PREFIX :        <http://w3id.org/probs-lab/ontology#>
PREFIX cc:      <http://creativecommons.org/ns#>
PREFIX dc:      <http://purl.org/dc/elements/1.1/>
PREFIX dcterms:	<http://purl.org/dc/terms/>
PREFIX foaf:    <http://xmlns.com/foaf/0.1/>
PREFIX gn:      <http://www.geonames.org/ontology#>
PREFIX obo:     <http://purl.obolibrary.org/obo/>
PREFIX org:     <http://www.w3.org/ns/org#>
PREFIX owl:     <http://www.w3.org/2002/07/owl#>
PREFIX prov:    <http://www.w3.org/ns/prov#>
PREFIX qudt:    <http://qudt.org/schema/qudt/>
PREFIX rdf:     <http://www.w3.org/1999/02/22-rdf-syntax-ns#>
PREFIX rdfs:    <http://www.w3.org/2000/01/rdf-schema#>
PREFIX time:    <http://www.w3.org/2006/time#>
PREFIX vann:    <http://purl.org/vocab/vann/>
PREFIX xsd:     <http://www.w3.org/2001/XMLSchema#>

<http://w3id.org/probs-lab/ontology>
    rdf:type            owl:Ontology ;

    vann:preferredNamespacePrefix   "probs" ;
    vann:preferredNamespaceUri      "http://w3id.org/probs-lab/ontology#" ;

    rdfs:label          "Physical Resources Observatory (PRObs) Ontology"@en ;
    dc:title            "Physical Resources Observatory (PRObs) Ontology"@en ;

    rdfs:comment        "The ontology describes entities useful for the development of the Physical Resources Observatory (PRObs) data integration system."@en ;
    dc:description      "The ontology describes entities useful for the development of the Physical Resources Observatory (PRObs) data integration system."@en ;

    dc:abstract         "Information about energy and material production and consumption is important for understanding issues such as decarbonisation of industry, recycling, and waste management. The Physical Resources Observatory (PRObs) ontology defines entities useful for describing and integrating this type of data. It reuses existing vocabularies for provenance (PROV), measurements (QUDT), time (OWL Time) and spatial regions (Geonames). It can be used to describe existing data, and as a basis to compute derived data aggregated according to different hierarchies."@en ;

    owl:versionIRI      <http://w3id.org/probs-lab/ontology-2.0.0> ;
    owl:versionInfo     "2.0.0" ;
    owl:priorVersion    <https://ukfires.org/probs/ontology-1.5.2> ;
    dcterms:created     "2020-10-02" ;
    dc:issued           "2020-10-02" ;
    dc:modified         "2023-01-27" ;

    dc:creator          "Stefano Germano" ;
    dc:creator          "Rick Lupton" ;
    dc:creator          "Carla Saunders" ;

    dc:contributor      "UK FIRES partners"@en ;

    cc:license          <https://creativecommons.org/licenses/by/4.0> .


#################################################################
#    Object Properties
#################################################################

:objectComposedOf
    rdf:type            owl:ObjectProperty ;
    rdfs:label          "object composed of"@en ;
    rdfs:comment        "Connects an Object to 'sub-Objects' lower in the hierarchy, which collectively exhaustively describe the same things."@en ;
    rdfs:domain         :Object ;
    rdfs:range          :Object .


:objectEquivalentTo
    rdf:type            owl:ObjectProperty ;
    rdf:type            owl:ReflexiveProperty ;
    rdf:type            owl:SymmetricProperty ;
    rdf:type            owl:TransitiveProperty ;
    rdfs:label          "object equivalent to"@en ;
    rdfs:comment        "Connects two Objects which describe exacly the same thing."@en ;
    vann:example        "Cement :objectEquivalentTo CementInCOMTRADE."@en ;
    rdfs:domain         :Object ;
    rdfs:range          :Object .


:partOfList
    rdf:type            owl:ObjectProperty ;
    rdf:type            owl:FunctionalProperty ;
    rdfs:label          "part of list"@en ;
    rdfs:comment        "Each ClassificationCode belongs to a ClassificationCodeList."@en ;
    vann:example        "10.11.11.40 :partOfList 2017PRODCOMlist"@en ;
    rdfs:domain         :ClassificationCode ;
    rdfs:range          :ClassificationCodeList .


:hasClassificationCode
    rdf:type            owl:ObjectProperty ;
    rdfs:label          "has classification code"@en ;
    rdfs:comment        "Links an Object to the ClassificationCode which describes it."@en ;
    vann:example        "Object10.11.11.40 :hasClassificationCode 10.11.11.40."@en ;
    rdfs:domain         :Object ;
    rdfs:range          :ClassificationCode .


:objectDefinedBy
    rdf:type            owl:ObjectProperty ;
    rdfs:label          "object defined by"@en ;
    rdfs:comment        "Links an Observation to the Object it describes."@en ;
    rdfs:domain         :Observation ;
    rdfs:range          :Object .


:objectDirectlyDefinedBy
    rdf:type            owl:ObjectProperty ;
    rdfs:subPropertyOf  :objectDefinedBy ;
    rdfs:label          "object directly defined by"@en ;
    rdfs:comment        "Links a direct Observation to the Object it describes."@en ;
    rdfs:domain         :DirectObservation ;
    rdfs:range          :Object .


:objectInferredDefinedBy
    rdf:type            owl:ObjectProperty ;
    rdfs:subPropertyOf  :objectDefinedBy ;
    rdfs:label          "object inferred defined by"@en ;
    rdfs:comment        "Links an inferred Observation to the Object it describes."@en ;
    rdfs:domain         :InferredObservation ;
    rdfs:range          :Object .


:processDefinedBy
    rdf:type            owl:ObjectProperty ;
    rdfs:label          "process defined by"@en ;
    rdfs:comment        "Links an Observation to the Process it describes."@en ;
    rdfs:domain         :Observation ;
    rdfs:range          :Process .


:processDirectlyDefinedBy
    rdf:type            owl:ObjectProperty ;
    rdfs:subPropertyOf  :processDefinedBy ;
    rdfs:label          "process directly defined by"@en ;
    rdfs:comment        "Links a direct Observation to the Process it describes."@en ;
    rdfs:domain         :DirectObservation ;
    rdfs:range          :Process .


:processInferredDefinedBy
    rdf:type            owl:ObjectProperty ;
    rdfs:subPropertyOf  :processDefinedBy ;
    rdfs:label          "process inferred defined by"@en ;
    rdfs:comment        "Links an inferred Observation to the Process it describes."@en ;
    rdfs:domain         :InferredObservation ;
    rdfs:range          :Process .


:hasTime
    rdf:type            owl:ObjectProperty ;
    rdf:type            owl:FunctionalProperty ;
    rdfs:label          "has time period"@en ;
    rdfs:comment        "Links an Observation to the Time in which it was measured."@en ;
    rdfs:domain         :Observation ;
    rdfs:range          time:TemporalEntity .


:hasRegion
    rdf:type            owl:ObjectProperty ;
    rdf:type            owl:FunctionalProperty ;
    rdfs:label          "has region"@en ;
    rdfs:comment        "Links an Observation to the Region in which it was measured."@en ;
    rdfs:domain         :Observation ;
    rdfs:range          gn:Feature .


:partOfDataset
    rdf:type            owl:ObjectProperty ;
    rdf:type            owl:FunctionalProperty ;
    rdfs:label          "part of dataset"@en ;
    rdfs:comment        "Links an Observation to the Dataset it is a part of."@en ;
    rdfs:domain         :Observation ;
    rdfs:range          :Dataset .


:processComposedOf
    rdf:type            owl:ObjectProperty ;
    rdfs:label          "process composed of"@en ;
    rdfs:comment        "Connects a Process to the 'sub-Processes' lower in the hierarchy, which collectively exhaustively describe the same activities."@en ;
    rdfs:domain         :Process ;
    rdfs:range          :Process .


:processEquivalentTo
    rdf:type            owl:ObjectProperty ;
    rdf:type            owl:ReflexiveProperty ;
    rdf:type            owl:SymmetricProperty ;
    rdf:type            owl:TransitiveProperty ;
    rdfs:label          "process equivalent to"@en ;
    rdfs:comment        "Connects two Processes which describe exacly the same thing."@en ;
    rdfs:domain         :Process ;
    rdfs:range          :Process .


:hasRole
    rdf:type            owl:ObjectProperty ;
    rdfs:label          "has role"@en ;
    rdfs:comment        "Links an Observation to the type of data represented by it."@en ;
    rdfs:domain         :Observation ;
    rdfs:range          :Role .


:consumes
    rdf:type            owl:ObjectProperty ;
    rdfs:label          "consumes"@en ;
    rdfs:comment        "Describes that an Object is an input to a Process."@en ;
    rdfs:domain         :Process ;
    rdfs:range          :Object .


:produces
    rdf:type            owl:ObjectProperty ;
    rdfs:label          "produces"@en ;
    rdfs:comment        "Describes that an Object is an output of a Process."@en ;
    rdfs:domain         :Process ;
    rdfs:range          :Object .


:hasMetric
    rdf:type            owl:ObjectProperty ;
    rdfs:label          "has metric"@en ;
    rdfs:comment        "The way in which a measurement is quantified (e.g. by mass, or by volume)."@en ;
    rdfs:domain         :Observation ;
    rdfs:range          qudt:QuantityKind .


:hasBound
    rdf:type            owl:ObjectProperty ;
    rdfs:label          "has bound"@en ;
    rdfs:comment        "Specifies the type of constraint that the Observation represents (exact/lower/upper bound)."@en ;
    rdfs:domain         :Observation ;
    rdfs:range          :MeasurementBound .


#################################################################
#    Data properties
#################################################################

:objectDescription
    rdf:type            owl:DatatypeProperty ;
    rdf:type            owl:FunctionalProperty ;
    rdfs:label          "object description"@en ;
    rdfs:comment        "Links an Object to a human-readable description of that Object."@en ;
    rdfs:domain         :Object ;
    rdfs:range          xsd:string .


:processDescription
    rdf:type            owl:DatatypeProperty ;
    rdf:type            owl:FunctionalProperty ;
    rdfs:label          "process description"@en ;
    rdfs:comment        "Links a Process to a human-readable description of that Object"@en ;
    rdfs:domain         :Process ;
    rdfs:range          xsd:string .


:codeDescription
    rdf:type            owl:DatatypeProperty ;
    rdf:type            owl:FunctionalProperty ;
    rdfs:label          "code description"@en ;
    rdfs:comment        "Links a ClassificationCode to a human-readable description, usually defined by the body which maintains the ClassificationCodeList."@en ;
    rdfs:domain         :ClassificationCode ;
    rdfs:range          xsd:string .


:measurement
    rdf:type            owl:DatatypeProperty ;
    rdf:type            owl:FunctionalProperty ;
    rdfs:label          "measurement"@en ;
    rdfs:comment        "The actual quantity of an Observation."@en ;
    rdfs:domain         :Observation ;
    rdfs:range          xsd:decimal .


#################################################################
#    Classes
#################################################################

:Object
    rdf:type            owl:Class ;
    rdfs:subClassOf     prov:Entity, obo:BFO_0000031 ;
    rdfs:label          "Object"@en ;
    rdfs:comment        "What is flowing in a Flow, or accumulated in a Stock. This is a more general term that includes Goods and Substances, but also non-material things such as energy and services."@en .


:ReferenceObject
    rdf:type            owl:Class ;
    rdfs:subClassOf     :Object ;
    rdfs:label          "ReferenceObject"@en ;
    rdfs:comment        "An Object type that has been purposefully defined as part of a description of the physical system (as opposed to some Object types that may be generated to encode more complex relationships)."@en .


:ClassificationCode
    rdf:type            owl:Class ;
    rdfs:label          "Classification code"@en ;
    rdfs:comment        "A label within a ClassificationCodeList."@en ;
    vann:example        "10.11.11.40 in the 2017-18 PRODCOM list."@en .


:ClassificationCodeList
    rdf:type            owl:Class ;
    rdfs:label          "Classification code list"@en ;
    rdfs:comment        "A set of ClassificationCodes."@en ;
    vann:example        "The 2017-18 PRODCOM list or the 2018 HS classification."@en .


:Observation
    rdf:type            owl:Class ;
    rdfs:subClassOf     obo:BFO_0000031 ;
    rdfs:subClassOf     prov:Entity ;
    rdfs:label          "Observation"@en ;
    rdfs:comment        "An individual observed data point."@en .


:Role
    rdf:type            owl:Class ;
    rdfs:subClassOf     obo:BFO_0000019 ;
    rdfs:label          "Role"@en ;
    rdfs:comment        "Type of data represented by an Observation."@en .


:Flow
    rdf:type            owl:Class ;
    rdfs:subClassOf     :Role ;
    rdfs:label          "Flow"@en ;
    rdfs:comment        "Movement of Objects across Process boundaries or between Regions."@en .


:SoldProduction
    rdf:type            owl:Class ;
    rdfs:subClassOf     :Flow ;
    rdfs:label          "Sold production"@en ;
    rdfs:comment        "A Flow which measures the total sold production of an Object. Defined by PRODCOM to exclude the goods that may have been produced within the factory boundary, but haven't yet left the factory gate."@en .


:Import
    rdf:type            owl:Class ;
    rdfs:subClassOf     :Flow ;
    rdfs:label          "Import"@en ;
    rdfs:comment        "A Flow which measures the quantity of an Object entering a Region."@en .


:Export
    rdf:type            owl:Class ;
    rdfs:subClassOf     :Flow ;
    rdfs:label          "Export"@en ;
    rdfs:comment        "A Flow which measures the quantity of an Object leaving a Region."@en .


:ProcessInput
    rdf:type            owl:Class ;
    rdfs:subClassOf     :Flow ;
    rdfs:label          "Process input"@en ;
    rdfs:comment        "A Flow which measures the input of a specific Object into a Process."@en .


:ProcessOutput
    rdf:type            owl:Class ;
    rdfs:subClassOf     :Flow ;
    rdfs:label          "Process output observation"@en ;
    rdfs:comment        "A Flow which describes the output of a specific Object from a Process."@en .


:Stock
    rdf:type            owl:Class ;
    rdfs:subClassOf     :Role ;
    rdfs:label          "Stock"@en ;
    rdfs:comment        "Accumulation of an Object within a Process."@en .


:DirectObservation
    rdf:type            owl:Class ;
    rdfs:subClassOf     :Observation ;
    rdfs:label          "Direct observation"@en ;
    rdfs:comment        "An Observation directly derived from data."@en .


:InferredObservation
    rdf:type            owl:Class ;
    rdfs:subClassOf     :Observation ;
    rdfs:label          "Inferred observation"@en ;
    rdfs:comment        "An Observation inferred from other Observations."@en .


:Process
    rdf:type            owl:Class ;
    rdfs:subClassOf     obo:BFO_0000031 ;
    rdfs:label          "Process"@en ;
    rdfs:comment        "One or more grouped operations in a system that can be defined and separated from others. A Process has an input of some Object(s) and an output of some Object(s)."@en .


:Dataset
    rdf:type            owl:Class ;
    rdfs:label          "Dataset"@en ;
    rdfs:comment        "A collection of Observations."@en ;
    vann:example        "The 2018 PRODCOM dataset."@en .


:MeasurementBound
    rdf:type            owl:Class ;
    rdfs:subClassOf     obo:BFO_0000019 ;
    rdfs:label          "Measurement bound"@en ;
    rdfs:comment        "The type of constraint that the Observation represents (exact/lower/upper bound)."@en .


#################################################################
#    Individuals
#################################################################

:LowerBound
    rdf:type            owl:NamedIndividual , :MeasurementBound ;
    rdfs:label          "Lower bound"@en ;
    rdfs:comment        "When an Observation has a LowerBound bound, it states that the true value is at least as great as the Observation's measurement."@en .


:UpperBound
    rdf:type            owl:NamedIndividual , :MeasurementBound ;
    rdfs:label          "Upper bound"@en ;
    rdfs:comment        "When an Observation has an UpperBound bound, it states that the true value is at most as great as the Observation's measurement."@en .


:ExactBound
    rdf:type            owl:NamedIndividual , :MeasurementBound ;
    rdfs:label          "Exact bound"@en ;
    rdfs:comment        "When an Observation has an ExactBound bound, it states that the true value is equal to the Observation's measurement."@en .


#################################################################
#    Annotations
#################################################################

<https://orcid.org/0000-0001-6993-0618>
    org:memberOf    [
                        foaf:name           "University of Oxford" ;
                        foaf:homepage       "https://www.ox.ac.uk"
                    ] ;
    foaf:name "Stefano Germano" .


<https://orcid.org/0000-0001-8622-3085>
    org:memberOf    [
                        foaf:name           "University of Bath" ;
                        foaf:homepage       "https://www.bath.ac.uk"
                    ] ;
    foaf:name "Rick Lupton" .


<https://orcid.org/0000-0001-6699-2848>
    org:memberOf    [
                        foaf:name           "University of Bath" ;
                        foaf:homepage       "https://www.bath.ac.uk"
                    ] ;
    foaf:name "Carla Saunders" .


#################################################################
#    Additional Axioms
#################################################################

 [] rdf:type            owl:AllDisjointClasses ;
    owl:members         (
                            :ClassificationCode
                            :Dataset
                            :MeasurementBound
                            :Object
                            :Observation
                            :Process
                            :Role
                        ) .
